%\newcommand{\pde}[2]{\frac{\partial #1}{\partial #2}}
%\newcommand{\sopde}[2]{\frac{\partial ^2 #1}{\partial #2 ^2}}
%\newcommand{\tvsopde}[3]{\frac{\partial^2 #1}{\partial #2 \partial #3}}

\section{Second Week}


\textbf{Example:} Find the solution $u$ of the PDE: $$ \pde{u(x)}{x_1} - \frac{1}{x_1^2}\pde{u(x)}{x_2} = 0 $$

For $x_1, x_2 > 0$ with the initial condition
\begin{center}
	$u(x) = x_1$ for  $x \in \Gamma$
\end{center}

where $$\Gamma = \{x \in \mathbb{R}^2 | x_1 = x_2, x_1, x_2 > 0\}.$$

\textbf{Solution:}

haha
